Foundation/Modal/ModalCompanion/Standard/Cl.lean
@@ -1,150 +1,88 @@
 module
 
 public import Foundation.Logic.Embedding
-public import Foundation.Modal.ModalCompanion.Standard.Int
+public import Foundation.Modal.Boxdot.GL_Grz
+public import Foundation.Modal.Kripke.Logic.S5
 public import Foundation.Modal.Kripke.Logic.S5Grz
+public import Foundation.Modal.ModalCompanion.Standard.Basic
 public import Foundation.Modal.Boxdot.Ver_Triv
--- public import Foundation.Propositional.Kripke.Logic.Cl
+public import Foundation.Propositional.Kripke.Hilbert.Cl
 
 @[expose] public section
 
-namespace LO.Modal
+namespace LO
 
 open LO.Entailment LO.Entailment.FiniteContext LO.Modal.Entailment
 open Propositional
-open Propositional.Formula (atom gödelTranslate)
+open Propositional.Formula (gödelTranslate)
 open Propositional.Logic (smallestMC largestMC)
 open Modal
 open Modal.Kripke
-open Modal.Formula.Kripke
 
-
-lemma smallestMC_of_Cl.mem_diabox_box : (Propositional.Cl.smallestMC) ⊢ (◇□(.atom 0) 🡒 □(.atom 0)) := by
-  have H₁ : (Propositional.Cl.smallestMC) ⊢ □(.atom 0) ⋎ □(∼□(.atom 0)) := by
-    apply Logic.sumNormal.mem₂!;
-    use Axioms.LEM (.atom 0);
-    constructor;
-    . apply Propositional.Logic.iff_provable.mp;
-      simp;
-    . tauto;
-  have H₂ : Propositional.Cl.smallestMC ⊢ ◇□(.atom 0) 🡒 ∼□(∼□(.atom 0)) := dia_duality!_mp;
-  cl_prover [H₁, H₂];
-
-instance : Entailment.HasAxiomFive (Propositional.Cl.smallestMC) where
-  Five φ := by
-    constructor;
-    apply Modal.Logic.iff_provable.mp;
-    apply Modal.Logic.subst (L := (Propositional.Cl.smallestMC)) (φ := Modal.Axioms.Five (.atom 0)) (s := λ a => φ);
-    have H₁ : Propositional.Cl.smallestMC ⊢ ◇□(∼.atom 0) 🡒 □(∼.atom 0) := Modal.Logic.subst (s := λ _ => ∼(.atom 0)) $ smallestMC_of_Cl.mem_diabox_box;
-    have H₂ : Propositional.Cl.smallestMC ⊢ ∼□◇(.atom 0) 🡒 ◇□(∼.atom 0) := dia_duality!_mp;
-    have H₃ : Propositional.Cl.smallestMC ⊢ ◇(.atom 0) 🡒 ∼□(∼.atom 0) := dia_duality!_mp;
-    cl_prover [H₁, H₂, H₃];
 
 namespace S5
 
-instance : Modal.S5 ≊ Propositional.Cl.smallestMC := by
-  apply Logic.equiv_of_provable;
-  intro φ;
-  constructor;
-  . intro hφ;
-    induction hφ using Modal.Hilbert.Normal.rec! with
-    | axm s h =>
-      rcases h with (rfl | rfl | rfl | rfl) <;> simp;
-    | mdp ihφψ ihφ => exact ihφψ ⨀ ihφ;
-    | nec ihφ => exact nec! ihφ;
-    | _ => simp;
-  . intro hφ;
-    induction hφ using Logic.sumNormal.rec! with
-    | mem₁ h => apply WeakerThan.pbl h;
-    | mdp ihφψ ihψ => exact ihφψ ⨀ ihψ;
-    | nec ihφ => exact nec! ihφ;
-    | subst ihφ => apply Logic.subst _ ihφ;
-    | mem₂ h =>
-      rcases h with ⟨φ, hφ, rfl⟩;
-      apply provable_gödelTranslated_of_provable ?_ (Propositional.Logic.iff_provable.mpr hφ);
-      rintro _ ⟨_, (rfl | rfl), ⟨s, rfl⟩⟩;
-      . simp;
-      . apply rm_diabox'!;
-        apply WeakerThan.pbl (𝓢 := Modal.S4);
-        apply (diaK'! $ gödelTranslated_axiomTc) ⨀ (iff_provable_Cl_provable_dia_gS4.mp _);
-        simp;
-
-lemma is_smallestMC_of_Cl : Modal.S5 = Propositional.Cl.smallestMC := Logic.eq_of_equiv
-
-instance : Sound (Propositional.Cl.smallestMC) FrameClass.S5 := Kripke.sound_frameClass_of_equiv Modal.S5 Propositional.Cl.smallestMC
-
-instance : ModalCompanion Propositional.Cl Modal.S5 := by
-  apply is_smallestMC_of_Cl ▸ Modal.instModalCompanion_of_smallestMC_via_KripkeSemantics
-    (IL := Propositional.Cl)
-    (IC := Propositional.Kripke.FrameClass.Cl)
-    (MC := Modal.Kripke.FrameClass.S5)
-  rintro F hF;
-  simp_all only [Set.mem_setOf_eq];
-  constructor;
+@[simp, grind .]
+lemma gödelTranslated_axiomLEM : Modal.S5 ⊢ (Axioms.LEM φ)ᵍ := by
+  apply Complete.complete (𝓜 := FrameClass.S5);
+  intro F hF V x;
+  replace hF := Set.mem_setOf_eq.mp hF;
+  apply Modal.Formula.Kripke.Satisfies.or_def.mpr;
+  apply or_iff_not_imp_left.mpr;
+  intro h y Rxy hφ;
+  apply h;
+  apply Modal.gödelTranslated_persistency hφ;
+  apply F.symm Rxy;
 
 end S5
 
 
-instance : Propositional.Cl.smallestMC ⪯ Modal.S5Grz := calc
-  _ ≊ Modal.S5    := by symm; infer_instance;
-  _ ⪯ Modal.S5Grz := inferInstance
+namespace Propositional.Cl
 
+lemma provable_S5_of_mem : φ ∈ Propositional.Cl → Modal.S5 ⊢ φᵍ := by
+  apply Propositional.Hilbert.provable_gödelTranslated_of_mem_logic;
+  rintro _ ⟨a, (⟨_, rfl⟩ | ⟨_, _, rfl⟩), rfl⟩ <;> simp;
 
-section S5Grz
+theorem modalCompanion_S5 : ModalCompanion Propositional.Cl Modal.S5 := by
+  apply modalCompanion_via_kripkeSemantics (P := λ F => IsRightEuclidean F);
+  . apply provable_S5_of_mem;
+  . intro φ;
+    apply Hilbert.Cl.instKripkeComplete.complete;
+  . rintro φ hφ F _ _;
+    apply Modal.instSoundLogicNatFormulaFrameClassS5S5.sound;
+    . grind;
+    . apply Set.mem_setOf_eq.mpr;
+      exact {};
 
+lemma provable_S5Grz_of_mem : φ ∈ Propositional.Cl → Modal.S5Grz ⊢ φᵍ := fun h ↦ WeakerThan.pbl $ provable_S5_of_mem h
 
-instance : Modal.S5Grz ≊ Propositional.Cl.largestMC := by
-  apply Logic.equiv_of_provable;
+theorem modalCompanion_S5Grz : ModalCompanion Propositional.Cl Modal.S5Grz := by
+  apply modalCompanion_via_kripkeSemantics (P := λ {κ} F => Finite κ ∧ Std.Symm F);
+  . apply provable_S5Grz_of_mem;
+  . intro φ;
+    apply Hilbert.Cl.instKripkeCompleteFinite.complete;
+  . rintro φ hφ F _ ⟨_, _⟩;
+    apply Logic.instSoundNatFormulaFrameClassS5GrzFinite_Triv.sound;
+    . grind;
+    . apply Set.mem_setOf_eq.mpr;
+      exact {};
+
+theorem modalCompanion_Triv : ModalCompanion Propositional.Cl Modal.Triv := by
   intro φ;
-  constructor;
-  . intro hφ;
-    induction hφ using Modal.Hilbert.Normal.rec! with
-    | axm _ h =>
-      rcases h with (rfl | rfl | rfl | rfl);
-      . simp;
-      . simp;
-      . apply WeakerThan.pbl (𝓢 := Propositional.Cl.smallestMC); simp;
-      . simp;
-    | mdp ihφψ ihψ => exact ihφψ ⨀ ihψ;
-    | nec ihφ => exact nec! ihφ;
-    | _ => apply Logic.sumNormal.mem₁!; simp;
-  . intro hφ;
-    induction hφ using Logic.sumNormal.rec! with
-    | mdp ihφψ ihψ => exact ihφψ ⨀ ihψ;
-    | subst ih => apply Logic.subst _ ih;
-    | nec ih => apply nec! ih;
-    | mem₁ h => apply WeakerThan.pbl h;
-    | mem₂ h => rcases h with ⟨φ, hφ, rfl⟩; simp;
+  apply Iff.trans modalCompanion_S5Grz;
+  apply Entailment.Equiv.iff.mp;
+  infer_instance;
 
-lemma is_largestMC_of_Cl : Modal.S5Grz = Propositional.Cl.largestMC := Logic.eq_of_equiv
+theorem boxdotModalCompanion_Ver : ∀ φ, φ ∈ Propositional.Cl ↔ Modal.Ver ⊢ φᵍᵇ :=
+  λ _ => Iff.trans modalCompanion_Triv $ Modal.Logic.iff_boxdotTranslated_Ver_Triv.symm
 
-instance : Sound Propositional.Cl.largestMC FrameClass.finite_Triv := Kripke.sound_frameClass_of_equiv Modal.S5Grz Propositional.Cl.largestMC
-
-end S5Grz
-
-
-instance S5Grz.modalCompanion : ModalCompanion Propositional.Cl Modal.S5Grz := by
-  apply is_largestMC_of_Cl ▸ Modal.instModalCompanion_of_largestMC_via_KripkeSemantics
-    (IC := Propositional.Kripke.FrameClass.finite_Cl)
-    (MC := Modal.Kripke.FrameClass.finite_Triv);
-  . intro F hF; simp_all only [Set.mem_setOf_eq]; exact {};
-
-instance Triv.modalCompanion : ModalCompanion Propositional.Cl Modal.Triv := by
-  convert S5Grz.modalCompanion;
-  have : Modal.Triv ≊ Modal.S5Grz := by symm; infer_instance;
-  apply Logic.eq_of_equiv;
-
-
-section boxdot
-
-theorem embedding_Cl_Ver {φ : Propositional.Formula ℕ} : Propositional.Cl ⊢ φ ↔ Modal.Ver ⊢ φᵍᵇ :=
-  Iff.trans ModalCompanion.companion Logic.iff_boxdotTranslated_Ver_Triv.symm
-
+/-
 instance : Entailment.FaithfullyEmbeddable Propositional.Cl Modal.Ver where
   prop := ⟨(·ᵍᵇ), fun _ ↦ embedding_Cl_Ver.symm⟩
+-/
 
-end boxdot
+end Propositional.Cl
 
+end LO
 
-end LO.Modal
 end
